disk-betree/ThreeStateVersionedMap.dfy
@@ -1,0 +1,6 @@
+include "ThreeStateVersioned.dfy"
+include "MapSpec.dfy"
+
+module ThreeStateVersionedMap refines ThreeStateVersioned {
+  import SM = MapSpec
+}
